src/impl/TLS13.Handshake.ByteDriver.External.fsti
@@ -3,8 +3,11 @@ module TLS13.Handshake.ByteDriver.External
 #lang-pulse
 
 open Pulse.Lib.Pervasives
+open Pulse.Lib.Array.PtsTo
 
+module B = TLS13.Bytes
 module IO = TLS13.IO
+module SZ = FStar.SizeT
 module U8 = FStar.UInt8
 
 type progress =
@@ -21,10 +24,37 @@ fn reset_encrypted_handshake (ctx: context)
   requires is_context ctx 'p
   ensures is_context ctx ExpectEncryptedExtensions
 
-fn read_next_encrypted_handshake_record (ctx: context) (ch: IO.channel)
+fn read_raw (ctx: context) (ch: IO.channel) (buf: array U8.t)
+  (total_len: SZ.t) (offset: SZ.t) (remaining: SZ.t)
   requires is_context ctx 'p ** IO.is_channel ch
+           ** pts_to buf 'old
+           ** pure (B.length 'old == SZ.v total_len /\
+                    SZ.v remaining > 0 /\
+                    SZ.v offset + SZ.v remaining <= SZ.v total_len)
+  returns n: SZ.t
+  ensures exists* bytes.
+          is_context ctx 'p ** IO.is_channel ch
+          ** pts_to buf bytes
+          ** pure (B.length bytes == SZ.v total_len /\
+                   SZ.v n <= SZ.v remaining)
+
+fn process_encrypted_handshake_record
+  (ctx: context)
+  (header: array U8.t)
+  (header_len: SZ.t)
+  (cipher: array U8.t)
+  (cipher_len: SZ.t)
+  requires is_context ctx 'p **
+           pts_to header 'header_bytes **
+           pts_to cipher 'cipher_bytes **
+           pure (B.length 'header_bytes == SZ.v header_len /\
+                 B.length 'cipher_bytes == SZ.v cipher_len /\
+                 SZ.v header_len == 5 /\
+                 SZ.v cipher_len > 16)
   returns ok: bool
-  ensures is_context ctx 'p ** IO.is_channel ch
+  ensures is_context ctx 'p **
+          pts_to header 'header_bytes **
+          pts_to cipher 'cipher_bytes
 
 fn pending_handshake_message_complete (ctx: context)
   requires is_context ctx 'p
